fv: add formal instance for point addition

fv/lean/Ragu/Instances/Point/AddIncomplete.lean
@@ -5,77 +5,130 @@ namespace Ragu.Instances.Point.AddIncomplete
 open Core.Primes
 
 @[reducible]
-def CircuitField := F Core.Primes.p
+def p := Core.Primes.p
 
-def Inputs := ProvableVector field 5
+@[reducible]
+def inputLen := 5
+
+@[reducible]
+def outputLen := 3
 
 set_option linter.unusedVariables false in
-def exported_operations (input_var : Var Inputs CircuitField) : Operations CircuitField := [
+def exportedOperations (input_var : Var (ProvableVector field inputLen) (F p)) : Operations (F p) := [
   Operation.witness 3 (fun _env => default),
-  Operation.assert ((((var 0) * (var 1)) + ((0x40000000000000000000000000000000224698fc094cf91b992d30ed00000000 : Expression CircuitField) * (var 2)))),
-  Operation.assert (((var 0) + ((0x40000000000000000000000000000000224698fc094cf91b992d30ed00000000 : Expression CircuitField) * (input_var.get 4)))),
-  Operation.assert (((var 1) + ((0x40000000000000000000000000000000224698fc094cf91b992d30ed00000000 : Expression CircuitField) * ((input_var.get 2) + ((0x40000000000000000000000000000000224698fc094cf91b992d30ed00000000 : Expression CircuitField) * (input_var.get 0)))))),
+  Operation.assert ((((var 0) * (var 1)) + ((0x40000000000000000000000000000000224698fc094cf91b992d30ed00000000 : Expression (F p)) * (var 2)))),
+  Operation.assert (((var 0) + ((0x40000000000000000000000000000000224698fc094cf91b992d30ed00000000 : Expression (F p)) * (input_var.get 4)))),
+  Operation.assert (((var 1) + ((0x40000000000000000000000000000000224698fc094cf91b992d30ed00000000 : Expression (F p)) * ((input_var.get 2) + ((0x40000000000000000000000000000000224698fc094cf91b992d30ed00000000 : Expression (F p)) * (input_var.get 0)))))),
   Operation.witness 3 (fun _env => default),
-  Operation.assert ((((var 3) * (var 4)) + ((0x40000000000000000000000000000000224698fc094cf91b992d30ed00000000 : Expression CircuitField) * (var 5)))),
-  Operation.assert ((((input_var.get 3) + ((0x40000000000000000000000000000000224698fc094cf91b992d30ed00000000 : Expression CircuitField) * (input_var.get 1))) + ((0x40000000000000000000000000000000224698fc094cf91b992d30ed00000000 : Expression CircuitField) * (var 5)))),
-  Operation.assert ((((input_var.get 2) + ((0x40000000000000000000000000000000224698fc094cf91b992d30ed00000000 : Expression CircuitField) * (input_var.get 0))) + ((0x40000000000000000000000000000000224698fc094cf91b992d30ed00000000 : Expression CircuitField) * (var 4)))),
+  Operation.assert ((((var 3) * (var 4)) + ((0x40000000000000000000000000000000224698fc094cf91b992d30ed00000000 : Expression (F p)) * (var 5)))),
+  Operation.assert ((((input_var.get 3) + ((0x40000000000000000000000000000000224698fc094cf91b992d30ed00000000 : Expression (F p)) * (input_var.get 1))) + ((0x40000000000000000000000000000000224698fc094cf91b992d30ed00000000 : Expression (F p)) * (var 5)))),
+  Operation.assert ((((input_var.get 2) + ((0x40000000000000000000000000000000224698fc094cf91b992d30ed00000000 : Expression (F p)) * (input_var.get 0))) + ((0x40000000000000000000000000000000224698fc094cf91b992d30ed00000000 : Expression (F p)) * (var 4)))),
   Operation.witness 3 (fun _env => default),
-  Operation.assert ((((var 6) * (var 7)) + ((0x40000000000000000000000000000000224698fc094cf91b992d30ed00000000 : Expression CircuitField) * (var 8)))),
-  Operation.assert (((var 6) + ((0x40000000000000000000000000000000224698fc094cf91b992d30ed00000000 : Expression CircuitField) * (var 3)))),
-  Operation.assert (((var 7) + ((0x40000000000000000000000000000000224698fc094cf91b992d30ed00000000 : Expression CircuitField) * (var 3)))),
+  Operation.assert ((((var 6) * (var 7)) + ((0x40000000000000000000000000000000224698fc094cf91b992d30ed00000000 : Expression (F p)) * (var 8)))),
+  Operation.assert (((var 6) + ((0x40000000000000000000000000000000224698fc094cf91b992d30ed00000000 : Expression (F p)) * (var 3)))),
+  Operation.assert (((var 7) + ((0x40000000000000000000000000000000224698fc094cf91b992d30ed00000000 : Expression (F p)) * (var 3)))),
   Operation.witness 3 (fun _env => default),
-  Operation.assert ((((var 9) * (var 10)) + ((0x40000000000000000000000000000000224698fc094cf91b992d30ed00000000 : Expression CircuitField) * (var 11)))),
-  Operation.assert (((var 9) + ((0x40000000000000000000000000000000224698fc094cf91b992d30ed00000000 : Expression CircuitField) * (var 3)))),
-  Operation.assert (((var 10) + ((0x40000000000000000000000000000000224698fc094cf91b992d30ed00000000 : Expression CircuitField) * ((input_var.get 0) + ((0x40000000000000000000000000000000224698fc094cf91b992d30ed00000000 : Expression CircuitField) * (((var 8) + ((0x40000000000000000000000000000000224698fc094cf91b992d30ed00000000 : Expression CircuitField) * (input_var.get 0))) + ((0x40000000000000000000000000000000224698fc094cf91b992d30ed00000000 : Expression CircuitField) * (input_var.get 2)))))))),
+  Operation.assert ((((var 9) * (var 10)) + ((0x40000000000000000000000000000000224698fc094cf91b992d30ed00000000 : Expression (F p)) * (var 11)))),
+  Operation.assert (((var 9) + ((0x40000000000000000000000000000000224698fc094cf91b992d30ed00000000 : Expression (F p)) * (var 3)))),
+  Operation.assert (((var 10) + ((0x40000000000000000000000000000000224698fc094cf91b992d30ed00000000 : Expression (F p)) * ((input_var.get 0) + ((0x40000000000000000000000000000000224698fc094cf91b992d30ed00000000 : Expression (F p)) * (((var 8) + ((0x40000000000000000000000000000000224698fc094cf91b992d30ed00000000 : Expression (F p)) * (input_var.get 0))) + ((0x40000000000000000000000000000000224698fc094cf91b992d30ed00000000 : Expression (F p)) * (input_var.get 2)))))))),
 ]
 
 set_option linter.unusedVariables false in
 @[reducible]
-def exported_output (input_var : Var Inputs CircuitField) : Vector (Expression CircuitField) 3 := #v[
-  (((var 8) + ((0x40000000000000000000000000000000224698fc094cf91b992d30ed00000000 : Expression CircuitField) * (input_var.get 0))) + ((0x40000000000000000000000000000000224698fc094cf91b992d30ed00000000 : Expression CircuitField) * (input_var.get 2))),
-  ((var 11) + ((0x40000000000000000000000000000000224698fc094cf91b992d30ed00000000 : Expression CircuitField) * (input_var.get 1))),
+def exportedOutput (input_var : Var (ProvableVector field inputLen) (F p)) : Vector (Expression (F p)) 3 := #v[
+  (((var 8) + ((0x40000000000000000000000000000000224698fc094cf91b992d30ed00000000 : Expression (F p)) * (input_var.get 0))) + ((0x40000000000000000000000000000000224698fc094cf91b992d30ed00000000 : Expression (F p)) * (input_var.get 2))),
+  ((var 11) + ((0x40000000000000000000000000000000224698fc094cf91b992d30ed00000000 : Expression (F p)) * (input_var.get 1))),
   (var 2),
 ]
 
-
 def circuit := Circuits.Point.AddIncomplete.circuit Circuits.Point.Spec.EpAffineParams (p:=Core.Primes.p)
 
-def deserializeInput (input : Var Inputs CircuitField) : Var Circuits.Point.AddIncomplete.Inputs CircuitField :=
+def deserializeInput (input : Var (ProvableVector field inputLen) (F p)) : Var Circuits.Point.AddIncomplete.Inputs (F p) :=
   {
     P1 := ⟨input.get 0, input.get 1⟩,
     P2 := ⟨input.get 2, input.get 3⟩,
     nonzero := input.get 4
   }
 
-def serializeOutput (outputs: Var Circuits.Point.AddIncomplete.Outputs CircuitField) : Vector (Expression CircuitField) 3 :=
+def serializeOutput (outputs: Var Circuits.Point.AddIncomplete.Outputs (F p)) : Vector (Expression (F p)) 3 :=
   #v[
     outputs.P3.x,
     outputs.P3.y,
     outputs.nonzero
   ]
 
-theorem same_circuit (input : Var Inputs CircuitField):
-    ((circuit (deserializeInput input)).operations 0).toFlat = (exported_operations input).toFlat := by
-  simp [Operations.toFlat, circuit_norm, FormalCircuit.toSubcircuit,
-    circuit, deserializeInput, exported_operations,
-    Circuits.Point.AddIncomplete.circuit, Circuits.Point.AddIncomplete.elaborated, Circuits.Point.AddIncomplete.main,
-    Circuits.Core.AllocMul.circuit, Circuits.Core.AllocMul.elaborated, Circuits.Core.AllocMul.main,
-    Circuits.Element.Square.circuit, Circuits.Element.Square.elaborated, Circuits.Element.Square.main,
-    Circuits.Element.DivNonzero.circuit, Circuits.Element.DivNonzero.elaborated, Circuits.Element.DivNonzero.main,
-    Circuits.Element.Mul.circuit, Circuits.Element.Mul.elaborated, Circuits.Element.Mul.main]
-  repeat (constructor; rfl)
-  constructor
+def formal_instance : Core.Statements.FormalInstance where
+  p
+  inputLen
+  outputLen
+  exportedOperations
+  exportedOutput
 
-theorem same_output (input : Var Inputs CircuitField) :
-    ((deserializeInput input) |> circuit |>.output 0 |> serializeOutput) = exported_output input:= by
-  simp [circuit_norm, FormalCircuit.toSubcircuit,
-    circuit, deserializeInput, serializeOutput,
-    Circuits.Point.AddIncomplete.circuit, Circuits.Point.AddIncomplete.elaborated, Circuits.Point.AddIncomplete.main,
-    Circuits.Core.AllocMul.circuit, Circuits.Core.AllocMul.elaborated, Circuits.Core.AllocMul.main,
-    Circuits.Element.Square.circuit, Circuits.Element.Square.elaborated, Circuits.Element.Square.main,
-    Circuits.Element.DivNonzero.circuit, Circuits.Element.DivNonzero.elaborated, Circuits.Element.DivNonzero.main,
-    Circuits.Element.Mul.circuit, Circuits.Element.Mul.elaborated, Circuits.Element.Mul.main]
-  repeat (constructor <;> congr)
+  Input := Circuits.Point.AddIncomplete.Inputs
+  Output := Circuits.Point.AddIncomplete.Outputs
+
+  deserializeInput
+  serializeOutput
+
+  Assumptions input :=
+    input.P1.isOnCurve Circuits.Point.Spec.EpAffineParams ∧ input.P2.isOnCurve Circuits.Point.Spec.EpAffineParams
+  Spec input output :=
+    let ⟨P1, P2, nonzero⟩ := input
+    (
+      -- If the x coordinates of P1 and P2 are different, then we can conclude that the
+      -- addition output is affine and is the correct result of the addition
+      P1.x ≠ P2.x -> (
+        (
+          match P1.add_incomplete P2  with
+          | none => False -- this case never happens
+          | some res => output.P3 = res
+        )
+        ∧ output.P3.isOnCurve Circuits.Point.Spec.EpAffineParams
+      )
+    ) ∧
+    (
+      -- if the x coordinates of P1 and P2 are equal, then output nonzero is 0
+      -- regardless of the input nonzero
+      (P1.x = P2.x -> output.nonzero = 0) ∧
+
+      -- if the x coordinates of P1 and P2 are not equal, then output nonzero preserves
+      -- non-zero-ness from input nonzero
+      (P1.x ≠ P2.x ->
+        (nonzero = 0 -> output.nonzero = 0) ∧
+        (nonzero ≠ 0 -> output.nonzero ≠ 0)
+      )
+    )
+
+
+  reimplementation := Circuits.Point.AddIncomplete.circuit Circuits.Point.Spec.EpAffineParams
+
+  same_circuit := by
+    intro input
+    simp [Operations.toFlat, circuit_norm, FormalCircuit.toSubcircuit,
+      deserializeInput, exportedOperations,
+      Circuits.Point.AddIncomplete.circuit, Circuits.Point.AddIncomplete.elaborated, Circuits.Point.AddIncomplete.main,
+      Circuits.Core.AllocMul.circuit, Circuits.Core.AllocMul.elaborated, Circuits.Core.AllocMul.main,
+      Circuits.Element.Square.circuit, Circuits.Element.Square.elaborated, Circuits.Element.Square.main,
+      Circuits.Element.DivNonzero.circuit, Circuits.Element.DivNonzero.elaborated, Circuits.Element.DivNonzero.main,
+      Circuits.Element.Mul.circuit, Circuits.Element.Mul.elaborated, Circuits.Element.Mul.main]
+    repeat (constructor; rfl)
+    constructor
+  same_output := by
+    intro input;
+    simp [circuit_norm, FormalCircuit.toSubcircuit,
+      deserializeInput, serializeOutput,
+      Circuits.Point.AddIncomplete.circuit, Circuits.Point.AddIncomplete.elaborated, Circuits.Point.AddIncomplete.main,
+      Circuits.Core.AllocMul.circuit, Circuits.Core.AllocMul.elaborated, Circuits.Core.AllocMul.main,
+      Circuits.Element.Square.circuit, Circuits.Element.Square.elaborated, Circuits.Element.Square.main,
+      Circuits.Element.DivNonzero.circuit, Circuits.Element.DivNonzero.elaborated, Circuits.Element.DivNonzero.main,
+      Circuits.Element.Mul.circuit, Circuits.Element.Mul.elaborated, Circuits.Element.Mul.main]
+    repeat (constructor <;> congr)
+  same_spec := by
+    intro input output;
+    simp [Circuits.Point.AddIncomplete.circuit, Circuits.Point.AddIncomplete.Spec]
+    intro h1 h2
+    aesop
+  same_assumptions := by intro input; rfl
 
 
 end Ragu.Instances.Point.AddIncomplete
